added bsim for running example

CompCertOC/concur/CallconvBig.v
@@ -1157,6 +1157,23 @@ Qed.
 
 End GS.
 
+Definition after_external_receptive (lts : semantics li_c li_c) : Prop :=
+  forall s q r se,
+    Smallstep.at_external (lts se) s q ->
+    exists s', Smallstep.after_external (lts se) s r s'.
+
+Definition initial_state_receptive (lts : semantics li_c li_c) : Prop :=
+  forall s vf sg args se m m',
+    Smallstep.initial_state (lts se) (cq vf sg args m) s ->
+    Mem.sup_include (Mem.support m) (Mem.support m') ->
+    exists s', Smallstep.initial_state (lts se) (cq vf sg args m') s'.
+
+Definition valid_query_receptive  (lts : semantics li_c li_c) : Prop :=
+  forall vf sg args se m m',
+    Smallstep.valid_query (lts se) (cq vf sg args m) =
+    Smallstep.valid_query (lts se) (cq vf sg args m').
+
+
 (** Transform the old callconv into new callconv with [world_unit], therefore new fsim is essentially the same as old one *)
 
 Import GS.
